src/Init/Data/Slice.lean
@@ -2,3 +2,4 @@ module
 
 prelude
 import Init.Data.Slice.Basic
+import Init.Data.Slice.Array
