tests/lean/run/slice.lean
@@ -1,0 +1,3 @@
+#eval (1..<2).toList
+
+#eval (Std.Slice.mk #[1, 2, 3] *..<2) |>.iter.toList
